template files

scripts/gen.py
@@ -1,10 +1,20 @@
 import jinja2
-import sys
+import argparse
+
+parser = argparse.ArgumentParser(description='templated memory abstractions')
+parser.add_argument('--base-width', type=int)
+parser.add_argument('--heaplet-width', type=int)
+parser.add_argument('--output-dir', type=str)
+args = parser.parse_args()
+
+# args = parser.parse_args('--base-width 32 --heaplet-width 256'.split())
 
 templateLoader = jinja2.FileSystemLoader(searchpath="./")
 templateEnv = jinja2.Environment(loader=templateLoader)
 
-BASE_WIDTH = 32
+base_width = args.base_width
+output_dir = args.output_dir
+assert(base_width % 8 == 0)
 
 class MemEntry():
     def __init__(self, num_bits, is_buff):
@@ -29,15 +39,23 @@ class MemEntry():
 
         self.align = self.num_bytes
         # how many base words to represent this word size
-        assert(self.num_bits % BASE_WIDTH == 0)
-        self.num_words = self.num_bits // BASE_WIDTH
+        assert(self.num_bits % base_width == 0)
+        self.num_words = self.num_bits // base_width
 
-single = MemEntry(BASE_WIDTH, False)
-buffer = MemEntry(256, True)
+single = MemEntry(base_width, False)
+buffer = MemEntry(args.heaplet_width, True)
 
-memory = templateEnv.get_template('mem.jinja2')
+with open(output_dir + "/flat.dfy", "w+") as f:
+    flat = templateEnv.get_template('flat.jinja2')
+    sizes = [single, buffer]
+    if single.num_bits == buffer.num_bits:
+        sizes = [single]
+    f.write(flat.render(base_size=single, sizes=sizes, limit="0x80000"))
 
-print(memory.render(base_size=single, sizes=[single, buffer], limit="0x80000"))
+with open(output_dir + "/stack.dfy", "w+") as f:
+    stack = templateEnv.get_template('stack.jinja2')
+    f.write(stack.render(base_size=single))
 
-heap = templateEnv.get_template('heap.jinja2')
-print(heap.render(base_size=single, buff_item=buffer, single_item=single))
+with open(output_dir + "/mem.dfy", "w+") as f:
+    mem = templateEnv.get_template('mem.jinja2')
+    f.write(mem.render(base_size=single, buff_item=buffer))
